<?xml version="1.0"?>
<rdf:RDF xmlns="http://purl.obolibrary.org/obo/omrse/dev/language.owl/"
     xml:base="http://purl.obolibrary.org/obo/omrse/dev/language.owl/"
     xmlns:dc="http://purl.org/dc/elements/1.1/"
     xmlns:obo="http://purl.obolibrary.org/obo/"
     xmlns:owl="http://www.w3.org/2002/07/owl#"
     xmlns:rdf="http://www.w3.org/1999/02/22-rdf-syntax-ns#"
     xmlns:xml="http://www.w3.org/XML/1998/namespace"
     xmlns:xsd="http://www.w3.org/2001/XMLSchema#"
     xmlns:foaf="http://xmlns.com/foaf/0.1/"
     xmlns:rdfs="http://www.w3.org/2000/01/rdf-schema#"
     xmlns:terms="http://purl.org/dc/terms/"
     xmlns:protege="http://protege.stanford.edu/plugins/owl/protege#"
     xmlns:oboInOwl="http://www.geneontology.org/formats/oboInOwl#">
    <owl:Ontology rdf:about="http://purl.obolibrary.org/obo/omrse/language.owl">
        <owl:imports rdf:resource="http://purl.obolibrary.org/obo/omrse/dev/omrse.owl"/>
        <dc:creator xml:lang="en">Mathias Brochhausen</dc:creator>
        <dc:creator xml:lang="en">Matthew Diller</dc:creator>
        <dc:creator xml:lang="en">S. Clint Dowland</dc:creator>
        <dc:creator xml:lang="en">William R. Hogan</dc:creator>
        <dc:title xml:lang="en">OMRSE Language</dc:title>
	<owl:versionInfo>2020-01-30</owl:versionInfo>
    </owl:Ontology>
    


    <!-- 
    ///////////////////////////////////////////////////////////////////////////////////////
    //
    // Annotation properties
    //
    ///////////////////////////////////////////////////////////////////////////////////////
     -->

    


    <!-- http://purl.obolibrary.org/obo/OMRSE_00002025 -->

    <owl:AnnotationProperty rdf:about="http://purl.obolibrary.org/obo/OMRSE_00002025">
        <rdfs:label xml:lang="en">ISO 639-1 code</rdfs:label>
    </owl:AnnotationProperty>
    


    <!-- http://purl.obolibrary.org/obo/OMRSE_00002026 -->

    <owl:AnnotationProperty rdf:about="http://purl.obolibrary.org/obo/OMRSE_00002026">
        <rdfs:label xml:lang="en">ISO 639-2/B code</rdfs:label>
    </owl:AnnotationProperty>
    


    <!-- http://purl.obolibrary.org/obo/OMRSE_00002027 -->

    <owl:AnnotationProperty rdf:about="http://purl.obolibrary.org/obo/OMRSE_00002027">
        <rdfs:label xml:lang="en">ISO 639-2/T code</rdfs:label>
    </owl:AnnotationProperty>
    


    <!-- http://purl.obolibrary.org/obo/OMRSE_00002028 -->

    <owl:AnnotationProperty rdf:about="http://purl.obolibrary.org/obo/OMRSE_00002028">
        <obo:IAO_0000111 xml:lang="en">ISO 639-3 code</obo:IAO_0000111>
    </owl:AnnotationProperty>
    


    <!-- 
    ///////////////////////////////////////////////////////////////////////////////////////
    //
    // Classes
    //
    ///////////////////////////////////////////////////////////////////////////////////////
     -->

    


    <!-- http://purl.obolibrary.org/obo/OMRSE_00000192 -->

    <owl:Class rdf:about="http://purl.obolibrary.org/obo/OMRSE_00000192">
        <rdfs:subClassOf rdf:resource="http://purl.obolibrary.org/obo/BFO_0000015"/>
        <obo:IAO_0000115 xml:lang="en">A process in which some participant shares some information content entity about some state of that participant with some other participant.</obo:IAO_0000115>
        <obo:IAO_0000117 xml:lang="en">Mathias Brochhausen</obo:IAO_0000117>
        <obo:IAO_0000117 xml:lang="en">Matthew Diller</obo:IAO_0000117>
        <obo:IAO_0000117 xml:lang="en">S. Clint Dowland</obo:IAO_0000117>
        <obo:IAO_0000117 xml:lang="en">William R. Hogan</obo:IAO_0000117>
        <rdfs:label xml:lang="en">communication</rdfs:label>
    </owl:Class>
    


    <!-- http://purl.obolibrary.org/obo/OMRSE_00000193 -->

    <owl:Class rdf:about="http://purl.obolibrary.org/obo/OMRSE_00000193">
        <rdfs:subClassOf rdf:resource="http://purl.obolibrary.org/obo/BFO_0000016"/>
        <obo:IAO_0000115 xml:lang="en">A disposition inhering in a material entity that, if realized, is realized by that material entityâ€™s communicating via some linguistic concretization.</obo:IAO_0000115>
        <obo:IAO_0000117 xml:lang="en">Mathias Brochhausen</obo:IAO_0000117>
        <obo:IAO_0000117 xml:lang="en">Matthew Diller</obo:IAO_0000117>
        <obo:IAO_0000117 xml:lang="en">S. Clint Dowland</obo:IAO_0000117>
        <obo:IAO_0000117 xml:lang="en">William R. Hogan</obo:IAO_0000117>
        <rdfs:label xml:lang="en">linguistic competence</rdfs:label>
    </owl:Class>
    


    <!-- http://purl.obolibrary.org/obo/OMRSE_00000194 -->

    <owl:Class rdf:about="http://purl.obolibrary.org/obo/OMRSE_00000194">
        <rdfs:subClassOf rdf:resource="http://purl.obolibrary.org/obo/BFO_0000016"/>
        <obo:IAO_0000115 xml:lang="en">A disposition inhering in a linguistic community that (i) is a maximal aggregate of communicatively compatible linguistic competences, and (ii) if realized, is realized by any and all realizations of those linguistic competences.</obo:IAO_0000115>
        <obo:IAO_0000117 xml:lang="en">Mathias Brochhausen</obo:IAO_0000117>
        <obo:IAO_0000117 xml:lang="en">Matthew Diller</obo:IAO_0000117>
        <obo:IAO_0000117 xml:lang="en">S. Clint Dowland</obo:IAO_0000117>
        <obo:IAO_0000117 xml:lang="en">William R. Hogan</obo:IAO_0000117>
        <rdfs:label xml:lang="en">language</rdfs:label>
    </owl:Class>
    


    <!-- http://purl.obolibrary.org/obo/OMRSE_00000195 -->

    <owl:Class rdf:about="http://purl.obolibrary.org/obo/OMRSE_00000195">
        <rdfs:subClassOf rdf:resource="http://purl.obolibrary.org/obo/BFO_0000040"/>
        <obo:IAO_0000115 xml:lang="en">A maximal aggregate of material entities such that each member bears a linguistic competence for the same language.</obo:IAO_0000115>
        <obo:IAO_0000117 xml:lang="en">Mathias Brochhausen</obo:IAO_0000117>
        <obo:IAO_0000117 xml:lang="en">Matthew Diller</obo:IAO_0000117>
        <obo:IAO_0000117 xml:lang="en">S. Clint Dowland</obo:IAO_0000117>
        <obo:IAO_0000117 xml:lang="en">William R. Hogan</obo:IAO_0000117>
        <rdfs:label xml:lang="en">linguistic community</rdfs:label>
    </owl:Class>
    


    <!-- http://purl.obolibrary.org/obo/OMRSE_00000196 -->

    <owl:Class rdf:about="http://purl.obolibrary.org/obo/OMRSE_00000196">
        <rdfs:subClassOf rdf:resource="http://purl.obolibrary.org/obo/IAO_0021003"/>
        <obo:IAO_0000115 xml:lang="en">A social act in which the active participant states a preference for some communicative process to be in a certain language.</obo:IAO_0000115>
        <obo:IAO_0000117 xml:lang="en">Mathias Brochhausen</obo:IAO_0000117>
        <obo:IAO_0000117 xml:lang="en">Matthew Diller</obo:IAO_0000117>
        <obo:IAO_0000117 xml:lang="en">S. Clint Dowland</obo:IAO_0000117>
        <obo:IAO_0000117 xml:lang="en">William R. Hogan</obo:IAO_0000117>
        <rdfs:label xml:lang="en">expression of preferred language</rdfs:label>
    </owl:Class>
    


    <!-- http://purl.obolibrary.org/obo/OMRSE_00000197 -->

    <owl:Class rdf:about="http://purl.obolibrary.org/obo/OMRSE_00000197">
        <rdfs:subClassOf rdf:resource="http://purl.obolibrary.org/obo/IAO_0000030"/>
        <obo:IAO_0000115 xml:lang="en">An information content entity that (i) is the specified output of an expression of preferred language; (ii) is about some person, some language, and some language competence; and (iii) conveys the language with which that person prefers to communicate within some given context.</obo:IAO_0000115>
        <obo:IAO_0000117 xml:lang="en">Mathias Brochhausen</obo:IAO_0000117>
        <obo:IAO_0000117 xml:lang="en">Matthew Diller</obo:IAO_0000117>
        <obo:IAO_0000117 xml:lang="en">S. Clint Dowland</obo:IAO_0000117>
        <obo:IAO_0000117 xml:lang="en">William R. Hogan</obo:IAO_0000117>
        <rdfs:label xml:lang="en">preferred language information content entity</rdfs:label>
    </owl:Class>
    

</rdf:RDF>



<!-- Generated by the OWL API (version 4.5.9.2019-02-01T07:24:44Z) https://github.com/owlcs/owlapi -->

